floyd-seq partially working

cprogs/mytest.c
@@ -1,0 +1,18 @@
+int is_leap_year(int year) {
+    //@ With year : Z,
+    /*@ Require
+      PROP (Int.min_signed <= year <= Int.max_signed)
+      LOCAL (temp _year (Vint (Int.repr year)))
+      SEP ()
+    */
+    /*@ Ensure
+      PROP ()
+      LOCAL (temp ret_temp (Val.of_bool (is_leap_year year)))
+      SEP ()
+    */
+    int a = year + 1;
+    int b = year % 4;
+    int c = year % 100;
+    int d = year % 400;
+    return b == 0 && c != 0 || d == 0;
+}
