frontend/ExportAClight.ml
@@ -635,9 +635,9 @@ let print_program p prog sourcefile normalized =
   Hashtbl.clear temp_names;
   name_program prog;
   fprintf p "@[<v 0>";
-  (* fprintf p "%s" prologue;
+  fprintf p "%s" prologue;
   List.iter (fprintf p "Require Import %s.@ ") !option_V;
-  print_clightgen_info p sourcefile normalized; *)
+  print_clightgen_info p sourcefile normalized;
   List.iter (print_globdef_annotation p) prog.Ctypes.prog_defs;
-  (* print_Gprog p prog.Ctypes.prog_defs; *)
+  print_Gprog p prog.Ctypes.prog_defs;
   fprintf p "@]@."
