floyd-seq/test_forward.v
@@ -1,1 +1,109 @@
-Require Import FloydSeq.forward.
+
+Require Import VST.floyd.proofauto.
+Require Import cprogs.append_prog.
+Require Import cprogs.append_def.
+Require Import FloydSeq.AClight.
+Import AClightNotations.
+
+Instance CompSpecs : compspecs. make_compspecs prog. Defined. 
+Definition Vprog : varspecs. mk_varspecs prog. Defined.
+
+Definition f_append_spec_annotation :=
+  ANNOTATION_WITH  sh x y s1 s2, ((
+       PROP(writable_share sh)
+       LOCAL (temp _x x; temp _y y)
+       SEP (listrep sh s1 x; listrep sh s2 y)),
+  (
+      EX r: val,
+       PROP()
+       LOCAL(temp ret_temp r)
+       SEP (listrep sh (s1++s2) r))).
+
+Definition f_append_spec_complex :=
+  ltac:(uncurry_funcspec f_append_spec_annotation).
+
+Definition f_append_funsig: funsig :=
+  (((_x, (tptr (Tstruct _list noattr))) ::
+    (_y, (tptr (Tstruct _list noattr))) :: nil),
+   (tptr (Tstruct _list noattr))).
+
+Definition append_spec :=
+  ltac:(make_funcspec _append f_append_funsig f_append_spec_complex).
+
+
+Definition Gprog : funspecs :=
+  ltac:(with_library prog [append_spec]).
+
+Locate start_function.
+Locate forward_if_tac.
+
+(* 
+Tactic Notation "forward_if" constr(post) :=
+  lazymatch type of post with
+  | Prop =>
+      match goal with
+      | |- semax _ (PROPx (?P) ?Q) _ _ =>
+      floyd.forward.forward_if_tac (PROPx (post :: P) Q)
+      end
+  | list Prop =>
+      match goal with
+      | |- semax _ (PROPx (?P) ?Q) _ _ =>
+          let P' := eval cbv iota zeta beta delta [app] in (post ++ P) in
+          floyd.forward.forward_if_tac (PROPx P' Q)
+      end
+  | localdef =>
+      match goal with
+      | |- semax _ (PROPx (?P) (LOCALx ?Q ?R)) _ _ =>
+          let Q' := remove_LOCAL2 constr:(cons post nil) Q in
+          floyd.forward.forward_if_tac (PROPx (P) (LOCALx (post :: Q') R))
+      end
+  | list localdef =>
+      match goal with
+      | |- semax _ (PROPx (?P) (LOCALx ?Q ?R)) _ _ =>
+          let Q' := remove_LOCAL2 post Q in
+          let Q'' := eval cbv iota zeta beta delta [app] in (post ++ Q') in
+          floyd.forward.forward_if_tac (PROPx (P) (LOCALx Q'' R))
+      end
+  | _ => floyd.forward.forward_if_tac post
+  end.
+
+Tactic Notation "forward_if" constr(post) :=
+  lazymatch type of post with
+  | Prop =>
+      match goal with
+      | |- semax _ (PROPx (?P) ?Q) _ _ =>
+          forward_if_tac (PROPx (post :: P) Q)
+      end
+  | list Prop =>
+      match goal with
+      | |- semax _ (PROPx (?P) ?Q) _ _ =>
+          let P' := eval cbv iota zeta beta delta [app] in (post ++ P) in
+          forward_if_tac (PROPx P' Q)
+      end
+  | localdef =>
+      match goal with
+      | |- semax _ (PROPx (?P) (LOCALx ?Q ?R)) _ _ =>
+          let Q' := remove_LOCAL2 constr:(cons post nil) Q in
+          forward_if_tac (PROPx (P) (LOCALx (post :: Q') R))
+      end
+  | list localdef =>
+      match goal with
+      | |- semax _ (PROPx (?P) (LOCALx ?Q ?R)) _ _ =>
+          let Q' := remove_LOCAL2 post Q in
+          let Q'' := eval cbv iota zeta beta delta [app] in (post ++ Q') in
+          forward_if_tac (PROPx (P) (LOCALx Q'' R))
+      end
+  | _ => forward_if_tac post
+  end. *)
+
+Lemma append_verif: 
+  semax_body Vprog Gprog f_append append_spec.
+Proof.
+  leaf_function.
+  floyd.forward.start_function.
+  forward_if.
+  forward.
+  admit.
+  forward.
+  
+
