floyd-seq/AClight.v
@@ -1,0 +1,121 @@
+Require Export VST.floyd.proofauto.
+Require Import FloydSeq.forward.
+(** ** Functions *)
+
+(** A function definition is composed of its return type ([fn_return]),
+  the names and types of its parameters ([fn_params]), the names
+  and types of its local variables ([fn_vars]), and the body of the
+  function (a statement, [fn_body]). *)
+
+Record function : Type := mkfunction {
+  fn_return: type;
+  fn_callconv: calling_convention;
+  fn_params: list (ident * type);
+  fn_vars: list (ident * type);
+  fn_temps: list (ident * type);
+  fn_body: statement
+}.
+
+Definition var_names (vars: list(ident * type)) : list ident :=
+  List.map (@fst ident type) vars.
+
+(** Functions can either be defined ([Internal]) or declared as
+  external functions ([External]). *)
+
+Definition fundef := Ctypes.fundef function.
+
+(** The type of a function definition. *)
+
+Definition type_of_function (f: function) : type :=
+  Tfunction (type_of_params (fn_params f)) (fn_return f) (fn_callconv f).
+
+Definition type_of_fundef (f: fundef) : type :=
+  match f with
+  | Internal fd => type_of_function fd
+  | External id args res cc => Tfunction args res cc
+  end.
+
+(** ** Programs *)
+
+(** As defined in module [Ctypes], a program, or compilation unit, is
+  composed of:
+- a list of definitions of functions and global variables;
+- the names of functions and global variables that are public (not static);
+- the name of the function that acts as entry point ("main" function).
+- a list of definitions for structure and union names
+- the corresponding composite environment
+- a proof that this environment is consistent with the definitions. *)
+
+Definition program := Ctypes.program function.
+
+(** Generate VST funcspec from annotation funcspec *)
+
+Ltac move_let_inside v :=
+  lazymatch goal with
+  | v := let (a, b) := _ in _ |- _ =>
+    lazymatch goal with
+    | v := let (a, b) := ?p in fun x:?T => ?content |- _ =>
+      let temp := fresh "temp" in
+      let x := fresh x in
+      refine (fun x => _);
+      pose (temp := (fun x:T => let (a, b) := p in content) x);
+      hnf in temp;
+      clear v;
+      rename temp into v;
+      move_let_inside v
+    | v := let (a, b) := ?p in (?pre, ?post) |- _ =>
+      exact (let (a, b) := p in pre, let (a, b) := p in post)
+    | _ => fail 0 v "is not recognized"
+    end
+  | _ => fail 0 v "must have form let (a, b) := p in _"
+  end.
+
+Ltac uncurry_funcspec spec :=
+  let spec_name := fresh "spec" in
+  let spec := eval unfold spec in spec in
+  pose (spec_name := spec);
+  repeat
+    lazymatch goal with
+    | spec_name := fun x:?T1 => fun y:?T2 => ?spec |- _ =>
+      first [ignore (T2 : _) | fail 2 "funcspec cannot have dependent type"];
+      first [
+        let spec_name1 := fresh "spec" in
+        pose (spec_name1 := (fun p : (T1*T2) => let (x, y) := p in spec));
+        clear spec_name;
+        rename spec_name1 into spec_name;
+        refine (let spec_name1 :=
+          ltac:(
+            match goal with
+            | spec_name := ?spec |- _ =>
+            let spec := eval unfold spec_name in spec_name in
+            let p := fresh "p" in
+            intro p;
+            pose (spec_name1 := spec p);
+            hnf in spec_name1;
+            clear spec_name;
+            rename spec_name1 into spec_name;
+            move_let_inside spec_name;
+            exact spec_name
+            end
+          ) in _);
+        clear spec_name;
+        rename spec_name1 into spec_name;
+        cbv beta zeta in spec_name
+      | fail 2 "Unknown error: failed to uncurry funcspec"
+      ]
+    end;
+  exact spec_name.
+
+Ltac make_funcspec name funsig spec :=
+  let spec := eval cbv beta zeta delta [spec] in spec in
+  lazymatch spec with
+  | fun x:?T => (?P, ?Q) =>
+    exact (name, NDmk_funspec funsig cc_default T (fun x => P) (fun x => Q))
+  | _ => fail 0 spec "is not in valid form of funcspec"
+  end.
+
+Module AClightNotations.
+Notation "'ANNOTATION_WITH' x .. y , c " :=
+  (fun x => .. (fun y => c) .. ) (at level 65, x binder, y binder).
+End AClightNotations.
+
