floyd-seq/test_leap.v
@@ -1,0 +1,48 @@
+
+Require Import VST.floyd.proofauto.
+Require Import cprogs.mytest_prog.
+Require Import cprogs.mytest_def.
+Require Import FloydSeq.AClight.
+Import AClightNotations.
+
+Instance CompSpecs : compspecs. make_compspecs prog. Defined. 
+Definition Vprog : varspecs. mk_varspecs prog. Defined.
+
+
+Definition f_is_leap_year_spec_annotation :=
+  ANNOTATION_WITH  year : Z, ((
+      PROP (Int.min_signed <= year <= Int.max_signed)
+      LOCAL (temp _year (Vint (Int.repr year)))
+      SEP ()),
+  (
+      PROP ()
+      LOCAL (temp ret_temp (Val.of_bool (is_leap_year year)))
+      SEP ())).
+
+Definition f_is_leap_year_spec_complex :=
+  ltac:(uncurry_funcspec f_is_leap_year_spec_annotation).
+
+Definition f_is_leap_year_funsig: funsig :=
+  (((_year, tint) :: nil), tint).
+
+Definition is_leap_year_spec :=
+  ltac:(make_funcspec _is_leap_year f_is_leap_year_funsig f_is_leap_year_spec_complex).
+
+Definition Gprog : funspecs :=
+  ltac:(with_library prog [is_leap_year_spec]).
+
+
+Lemma append_verif: 
+  semax_body Vprog Gprog f_is_leap_year is_leap_year_spec.
+Proof.
+  leaf_function.
+  floyd.forward.start_function.
+  forward.
+  admit.
+  forward. admit.
+  forward. admit.
+  forward. admit.
+  forward_if. admit.
+  
+
+
